\documentclass{article}
\usepackage{amsmath}
\usepackage{amssymb}
\usepackage{logicproof}

\begin{document}

\begin{center}
\section*{Some submission}
\end{center}

\subsection*{Sequent}
\begin{center}
$\exists  x (P \land  Q), \exists  x (P \land  \forall  y (P \rightarrow  x=y)) \vdash \forall  x (P \rightarrow  Q)$
\end{center}

\subsection*{Proof}
\begin{logicproof}{4}
\exists  x (P \land  Q) & premise \\
\exists  x (P \land  \forall  y (P \rightarrow  x=y)) & premise \\
\begin{subproof}
x_0 & $\mathrm{free}$  \\
\begin{subproof}
P & $\mathrm{assumption}$  \\
\begin{subproof}
x_1 & $\mathrm{free}$  \\
P \land  Q & $\mathrm{assumption}$  \\
P & $\land \mathrm{EL}$ 6 \\
Q & $\land \mathrm{ER}$ 6 \\
\begin{subproof}
x_2 & $\mathrm{free}$  \\
P \land  \forall  y (P \rightarrow  x_2=y) & $\mathrm{assumption}$  \\
\forall  y (P \rightarrow  x_2=y) & $\land \mathrm{ER}$ 10 \\
P \rightarrow  x_2=x_0 & $\forall \mathrm{E}$ 11, x_0 \\
x_2=x_0 & $\rightarrow \mathrm{E}$ 12, 4 \\
P \rightarrow  x_2=x_1 & $\forall \mathrm{E}$ 11, x_1 \\
x_2=x_1 & $\rightarrow \mathrm{E}$ 14, 7 \\
x_2=x_2 & $= \mathrm{I}$  \\
x_1=x_2 & $= \mathrm{E}$ 15, 16, u:=u=x_2 \\
x_1=x_0 & $= \mathrm{E}$ 13, 17, u:=x_1=u \\
Q & $= \mathrm{E}$ 18, 8, u:=Q
\end{subproof}
Q & $\exists \mathrm{E}$ 2, 9-19
\end{subproof}
Q & $\exists \mathrm{E}$ 1, 5-20
\end{subproof}
P \rightarrow  Q & $\rightarrow \mathrm{I}$ 4-21
\end{subproof}
\forall  x (P \rightarrow  Q) & $\forall \mathrm{I}$ 3-22
\end{logicproof}


\end{document}
